Derive a few Hoare triples about toycpu

toy-models/decompiler/prog_toyLib.sig
@@ -1,0 +1,8 @@
+signature prog_toyLib =
+sig
+
+    include helperLib
+
+    val toy_tools            : decompiler_tools
+
+end
