toy-models/decompiler/prog_toyLib.sml
@@ -1,0 +1,64 @@
+structure prog_toyLib :> prog_toyLib =
+struct
+
+open HolKernel boolLib bossLib;
+open wordsLib stringLib addressTheory pred_setTheory combinTheory;
+open set_sepTheory prog_toyTheory helperLib wordsTheory progTheory
+     finite_mapTheory decompilerLib;
+
+val toy_status = tFlags_HIDE;
+val toy_pc = ``PC``;
+fun toy_jump tm1 tm2 jump_length forward = ("",1)
+
+val lemmas = [ILOAD',ILOAD,ISTORE',ISTORE,MOV_CNST,MOV_REG]
+
+fun toy_spec s = let
+  val tm = Term [QUOTE s]
+  (* find right lemma *)
+  fun inst_lemma lemma = let
+    val pat = lemma |> concl |> rator |> rand |> rator |> rand |> rand
+    val i = fst (match_term pat tm)
+    in INST i lemma end
+  val th = inst_lemma (first (can inst_lemma) lemmas)
+  (* fix reg names *)
+  val tms = find_terms (can (match_term ``tReg x y``)) (concl th |> rator)
+  fun renamer tm = let
+    val y = rand tm
+    val x = rator tm |> rand |> rand |> numSyntax.int_of_term |> int_to_string
+    in y |-> mk_var("r" ^ x,type_of y) end
+  val th = INST (map renamer tms) th
+  in ((th,1,SOME 1),NONE) end
+
+val toy_tools =
+  ((toy_spec, toy_jump, toy_status, toy_pc):decompiler_tools);
+
+fun custom_set_pc i th =
+  INST [mk_var("p",``:num``) |-> ``p + ^(numSyntax.term_of_int i)``]
+    (th |> SIMP_RULE std_ss [GSYM arithmeticTheory.ADD_ASSOC])
+
+val _ = (decompiler_set_pc := custom_set_pc);
+
+val q = helperLib.quote_to_strings
+val tools = toy_tools
+val name = "test"
+val code = `
+  ILOAD 1w 2w
+  MOV 2w (CNST 2w)
+`
+
+(*
+  decompile tools name code
+*)
+
+
+(*
+
+  toy_spec "ILOAD 2w 3w"
+  toy_spec "ILOAD 3w 3w"
+  toy_spec "ISTORE 1w 2w"
+  toy_spec "MOV 1w (REG 2w)"
+  toy_spec "MOV 1w (CNST 2w)"
+
+*)
+
+end
