toy-models/decompiler/prog_toyScript.sml
@@ -1,0 +1,443 @@
+
+open HolKernel boolLib bossLib Parse;
+open pred_setTheory res_quanTheory wordsTheory wordsLib bitTheory arithmeticTheory;
+open listTheory pairTheory combinTheory addressTheory finite_mapTheory set_sepTheory;
+
+open toycpuTheory progTheory;
+
+val _ = new_theory "prog_toy";
+val _ = tight_equality();
+
+val RW = REWRITE_RULE;
+val RW1 = ONCE_REWRITE_RULE;
+
+
+(* ----------------------------------------------------------------------------- *)
+(* The TOY set                                                                   *)
+(* ----------------------------------------------------------------------------- *)
+
+val _ = Datatype `
+  toy_el = Runstate runstate
+         | PC num
+         | Inst num (instruction option)
+         | Reg word2 word64
+         | Flag flag bool
+         | Context (addr -> α -> (value # α) option)
+                   (addr -> value -> α -> α option) α
+`
+
+val toy_el_11 = DB.fetch "-" "toy_el_11";
+val toy_el_distinct = DB.fetch "-" "toy_el_distinct";
+
+val _ = Parse.type_abbrev("toy_set",``:('a toy_el) set``);
+
+
+(* ----------------------------------------------------------------------------- *)
+(* Converting from TOY-state record to toy_set                                   *)
+(* ----------------------------------------------------------------------------- *)
+
+val toy_read_reg_def = Define `
+  toy_read_reg (n:word2) s = s.registers ' (w2n n)`
+
+val toy_read_flag_def = Define `
+  toy_read_flag n s = s.flags n`
+
+val toy_read_inst_def = Define `
+  toy_read_inst n s =
+    if n < LENGTH s.instructions then SOME (EL n s.instructions) else NONE`
+
+val toy2set'_def = Define `
+  toy2set' (rs,pc,is,rg,fl,cc) (s:'a cpustate) =
+    (if rs then { Runstate s.runstate } else {}) UNION
+    (if pc then { PC s.pc } else {}) UNION
+    IMAGE (\a. Inst a (toy_read_inst a s)) is UNION
+    IMAGE (\a. Reg a (toy_read_reg a s)) rg UNION
+    IMAGE (\a. Flag a (toy_read_flag a s)) fl UNION
+    (if cc then { Context s.mload s.mstore s.context } else {})`;
+
+val toy2set_def   = Define `toy2set s = toy2set' (T,T,UNIV,UNIV,UNIV,T) s`;
+val toy2set''_def = Define `toy2set'' x s = toy2set s DIFF toy2set' x s`;
+
+(* theorems *)
+
+val toy2set'_SUBSET_toy2set = prove(
+  ``!y s. toy2set' y s SUBSET toy2set s``,
+  strip_tac
+  \\ PairCases_on `y`
+  \\ SIMP_TAC std_ss [SUBSET_DEF,toy2set'_def,toy2set_def,IN_IMAGE,IN_UNION,IN_UNIV]
+  \\ METIS_TAC [NOT_IN_EMPTY]);
+
+val SPLIT_toy2set = prove(
+  ``!x s. SPLIT (toy2set s) (toy2set' x s, toy2set'' x s)``,
+  REPEAT STRIP_TAC
+  \\ ASM_SIMP_TAC std_ss [SPLIT_def,EXTENSION,IN_UNION,IN_DIFF,toy2set''_def]
+  \\ `toy2set' x s SUBSET toy2set s` by METIS_TAC [toy2set'_SUBSET_toy2set]
+  \\ SIMP_TAC bool_ss [DISJOINT_DEF,EXTENSION,IN_INTER,NOT_IN_EMPTY,IN_DIFF]
+  \\ METIS_TAC [SUBSET_DEF]);
+
+val PUSH_IN_INTO_IF = METIS_PROVE []
+  ``!g x y z. (x IN (if g then y else z)) = if g then x IN y else x IN z``;
+
+val SUBSET_toy2set = prove(
+  ``!u s. (u SUBSET toy2set s) = ?y. u = toy2set' y s``,
+  REPEAT STRIP_TAC \\ EQ_TAC \\ REPEAT STRIP_TAC
+  \\ ASM_REWRITE_TAC [toy2set'_SUBSET_toy2set]
+  \\ Q.EXISTS_TAC `
+       ((?y. Runstate y IN u),
+        (?y. PC y IN u),
+        { a |a| ?x. Inst a x IN u },
+        { a |a| ?x. Reg a x IN u },
+        { a |a| ?x. Flag a x IN u },
+        (?y1 y2 y3. Context y1 y2 y3 IN u))`
+  \\ FULL_SIMP_TAC std_ss [toy2set'_def,toy2set_def,EXTENSION,SUBSET_DEF,IN_IMAGE,
+       IN_UNION,GSPECIFICATION,IN_INSERT,NOT_IN_EMPTY,IN_UNIV,PUSH_IN_INTO_IF]
+  \\ STRIP_TAC \\ ASM_REWRITE_TAC [] \\ EQ_TAC \\ REPEAT STRIP_TAC THEN1 METIS_TAC []
+  \\ PAT_X_ASSUM ``!x:'a. b:bool`` (IMP_RES_TAC)
+  \\ FULL_SIMP_TAC std_ss [toy_el_11,toy_el_distinct]);
+
+val SPLIT_toy2set_EXISTS = prove(
+  ``!s u v. SPLIT (toy2set s) (u,v) = ?y. (u = toy2set' y s) /\ (v = toy2set'' y s)``,
+  REPEAT STRIP_TAC \\ EQ_TAC \\ REPEAT STRIP_TAC \\ ASM_REWRITE_TAC [SPLIT_toy2set]
+  \\ FULL_SIMP_TAC bool_ss [SPLIT_def,toy2set'_def,toy2set''_def]
+  \\ `u SUBSET (toy2set s)` by
+       (FULL_SIMP_TAC std_ss [EXTENSION,SUBSET_DEF,IN_UNION] \\ METIS_TAC [])
+  \\ FULL_SIMP_TAC std_ss [SUBSET_toy2set] \\ Q.EXISTS_TAC `y` \\ REWRITE_TAC []
+  \\ fs [EXTENSION,IN_DIFF,IN_UNION,DISJOINT_DEF,NOT_IN_EMPTY,IN_INTER]
+  \\ METIS_TAC []);
+
+val IN_toy2set = store_thm("IN_toy2set[simp]",``
+  (!x s. Runstate x IN (toy2set s) <=> (x = s.runstate)) /\
+  (!x s. Runstate x IN (toy2set' (rs,pc,is,rg,fl,cc) s) <=> (x = s.runstate) /\ rs) /\
+  (!x s. Runstate x IN (toy2set'' (rs,pc,is,rg,fl,cc) s) <=> (x = s.runstate) /\ ~rs) /\
+  (!x s. PC x IN (toy2set s) <=> (x = s.pc)) /\
+  (!x s. PC x IN (toy2set' (rs,pc,is,rg,fl,cc) s) <=> (x = s.pc) /\ pc) /\
+  (!x s. PC x IN (toy2set'' (rs,pc,is,rg,fl,cc) s) <=> (x = s.pc) /\ ~pc) /\
+  (!a x s. Inst a x IN (toy2set s) <=> (x = toy_read_inst a s)) /\
+  (!a x s. Inst a x IN (toy2set' (rs,pc,is,rg,fl,cc) s) <=> (x = toy_read_inst a s) /\ a IN is) /\
+  (!a x s. Inst a x IN (toy2set'' (rs,pc,is,rg,fl,cc) s) <=> (x = toy_read_inst a s) /\ ~(a IN is)) /\
+  (!a x s. Reg a x IN (toy2set s) <=> (x = toy_read_reg a s)) /\
+  (!a x s. Reg a x IN (toy2set' (rs,pc,is,rg,fl,cc) s) <=> (x = toy_read_reg a s) /\ a IN rg) /\
+  (!a x s. Reg a x IN (toy2set'' (rs,pc,is,rg,fl,cc) s) <=> (x = toy_read_reg a s) /\ ~(a IN rg)) /\
+  (!a x s. Flag a x IN (toy2set s) <=> (x = toy_read_flag a s)) /\
+  (!a x s. Flag a x IN (toy2set' (rs,pc,is,rg,fl,cc) s) <=> (x = toy_read_flag a s) /\ a IN fl) /\
+  (!a x s. Flag a x IN (toy2set'' (rs,pc,is,rg,fl,cc) s) <=> (x = toy_read_flag a s) /\ ~(a IN fl)) /\
+  (!x1 x2 x3 s. Context x1 x2 x3 IN (toy2set s) <=>
+                x1 = s.mload /\ x2 = s.mstore /\ x3 = s.context) /\
+  (!x1 x2 x3 s. Context x1 x2 x3 IN (toy2set' (rs,pc,is,rg,fl,cc) s) <=>
+                x1 = s.mload /\ x2 = s.mstore /\ x3 = s.context /\ cc) /\
+  (!x1 x2 x3 s. Context x1 x2 x3 IN (toy2set'' (rs,pc,is,rg,fl,cc) s) <=>
+                x1 = s.mload /\ x2 = s.mstore /\ x3 = s.context /\ ~cc)``,
+  SRW_TAC [] [toy2set'_def,toy2set''_def,toy2set_def,IN_UNION,
+     IN_INSERT,NOT_IN_EMPTY,IN_DIFF,PUSH_IN_INTO_IF] \\ METIS_TAC []);
+
+val toy2set''_11 = prove(
+  ``!y y' s s'. (toy2set'' y' s' = toy2set'' y s) ==> (y = y')``,
+  REPEAT STRIP_TAC \\ CCONTR_TAC
+  \\ PairCases_on `y` \\ PairCases_on `y'`
+  \\ rename1 `(rs,pc,is,rg,fl,cc) <> (rs',pc',is',rg',fl',cc')`
+  \\ fs []
+  THEN1
+   (`(?x. Runstate x IN toy2set'' (rs,pc,is,rg,fl,cc) s) <>
+     (?x. Runstate x IN toy2set'' (rs',pc',is',rg',fl',cc') s')` by fs []
+    \\ rev_full_simp_tac std_ss [])
+  THEN1
+   (`(?x. PC x IN toy2set'' (rs,pc,is,rg,fl,cc) s) <>
+     (?x. PC x IN toy2set'' (rs',pc',is',rg',fl',cc') s')` by fs []
+    \\ rev_full_simp_tac std_ss [])
+  THEN1
+   (`?a. ~(a IN is <=> a IN is')` by METIS_TAC [EXTENSION]
+    \\ `(?x. Inst a x IN toy2set'' (rs,pc,is,rg,fl,cc) s) <>
+        (?x. Inst a x IN toy2set'' (rs',pc',is',rg',fl',cc') s')` by fs []
+    \\ rev_full_simp_tac std_ss [])
+  THEN1
+   (`?a. ~(a IN rg <=> a IN rg')` by METIS_TAC [EXTENSION]
+    \\ `(?x. Reg a x IN toy2set'' (rs,pc,is,rg,fl,cc) s) <>
+        (?x. Reg a x IN toy2set'' (rs',pc',is',rg',fl',cc') s')` by fs []
+    \\ rev_full_simp_tac std_ss [])
+  THEN1
+   (`?a. ~(a IN fl <=> a IN fl')` by METIS_TAC [EXTENSION]
+    \\ `(?x. Flag a x IN toy2set'' (rs,pc,is,rg,fl,cc) s) <>
+        (?x. Flag a x IN toy2set'' (rs',pc',is',rg',fl',cc') s')` by fs []
+    \\ rev_full_simp_tac std_ss [])
+  THEN1
+   (`(?x1 x2 x3. Context x1 x2 x3 IN toy2set'' (rs,pc,is,rg,fl,cc) s) <>
+     (?x1 x2 x3. Context x1 x2 x3 IN toy2set'' (rs',pc',is',rg',fl',cc') s')` by fs []
+    \\ rev_full_simp_tac std_ss []));
+
+val DELETE_toy2set = store_thm("DELETE_toy2set[simp]",``
+  (!s. (toy2set' (rs,pc,is,rg,fl,cc) s) DELETE Runstate (s.runstate) =
+       (toy2set' (F,pc,is,rg,fl,cc) s)) /\
+  (!s. (toy2set' (rs,pc,is,rg,fl,cc) s) DELETE PC (s.pc) =
+       (toy2set' (rs,F,is,rg,fl,cc) s)) /\
+  (!s. (toy2set' (rs,pc,is,rg,fl,cc) s) DELETE Inst i (toy_read_inst i s) =
+       (toy2set' (rs,pc,is DELETE i,rg,fl,cc) s)) /\
+  (!s. (toy2set' (rs,pc,is,rg,fl,cc) s) DELETE Reg r (toy_read_reg r s) =
+       (toy2set' (rs,pc,is,rg DELETE r,fl,cc) s)) /\
+  (!s. (toy2set' (rs,pc,is,rg,fl,cc) s) DELETE Flag f (toy_read_flag f s) =
+       (toy2set' (rs,pc,is,rg,fl DELETE f,cc) s)) /\
+  (!s. (toy2set' (rs,pc,is,rg,fl,cc) s) DELETE Context s.mload s.mstore s.context =
+       (toy2set' (rs,pc,is,rg,fl,F) s))``,
+  SRW_TAC [] [toy2set'_def,EXTENSION,IN_UNION,GSPECIFICATION,LEFT_AND_OVER_OR,
+    EXISTS_OR_THM,IN_DELETE,IN_INSERT,NOT_IN_EMPTY,PUSH_IN_INTO_IF]
+  \\ Cases_on `x` \\ SRW_TAC [] [] \\ METIS_TAC []);
+
+val EMPTY_toy2set = store_thm("EMPTY_toy2set[simp]",``
+  (toy2set' (rs,pc,is,rg,fl,cc) s = {}) <=>
+  ~rs /\ ~pc /\ is = {} /\ rg = {} /\ fl = {} /\ ~cc``,
+  Cases_on `rs` THEN1 fs [toy2set'_def]
+  \\ Cases_on `pc` THEN1 fs [toy2set'_def]
+  \\ Cases_on `cc` THEN1 fs [toy2set'_def]
+  \\ fs [toy2set'_def] \\ metis_tac []);
+
+
+(* ----------------------------------------------------------------------------- *)
+(* Defining the TOY_MODEL                                                        *)
+(* ----------------------------------------------------------------------------- *)
+
+val tRunstate_def = Define `tRunstate x = SEP_EQ { Runstate x }`
+val tPC_def = Define `tPC x = SEP_EQ { PC x }`
+val tInst_def = Define `tInst i x = SEP_EQ { Inst i x }`
+val tReg_def = Define `tReg i x = SEP_EQ { Reg i x }`
+val tFlag_def = Define `tFlag i x = SEP_EQ { Flag i x }`
+val tContext_def = Define `tContext x1 x2 x3 = SEP_EQ { Context x1 x2 x3 }`
+
+val Flags_def = Define `tFlags (zf,posf) = tFlag ZF zf * tFlag SF posf`;
+
+val TOY_NEXT_REL_def = Define `
+  TOY_NEXT_REL s s' = (step s = s')`;
+
+val TOY_INSTR_def = Define `
+  TOY_INSTR (a,w) = {(Inst a (SOME w))}`;
+
+val tm = rand ``SPEC (toy2set,
+                      TOY_NEXT_REL,
+                      TOY_INSTR,
+                      (\x y. x = (y:'a cpustate)),
+                      ((K F):('a cpustate) -> bool))``
+
+val TOY_MODEL_def = Define `
+  TOY_MODEL = ^tm`;
+
+(* theorems *)
+
+val lemma =
+  METIS_PROVE [SPLIT_toy2set]
+  ``p (toy2set' y s) ==>
+    (?u v. SPLIT (toy2set s) (u,v) /\ p u /\ (\v. v = toy2set'' y s) v)``;
+
+val TOY_SPEC_SEMANTICS = store_thm("TOY_SPEC_SEMANTICS",
+  ``SPEC TOY_MODEL p {} q =
+    !y s seq. p (toy2set' y s) /\ rel_sequence TOY_NEXT_REL seq s ==>
+              ?k. q (toy2set' y (seq k)) /\ (toy2set'' y s = toy2set'' y (seq k))``,
+  SIMP_TAC std_ss [GSYM RUN_EQ_SPEC,RUN_def,TOY_MODEL_def,STAR_def,SEP_REFINE_def]
+  \\ REPEAT STRIP_TAC \\ REVERSE EQ_TAC \\ REPEAT STRIP_TAC
+  THEN1 (FULL_SIMP_TAC bool_ss [SPLIT_toy2set_EXISTS] \\ METIS_TAC [])
+  \\ Q.PAT_X_ASSUM `!s r. b` (STRIP_ASSUME_TAC o UNDISCH o SPEC_ALL o
+     (fn th => MATCH_MP th (UNDISCH lemma)) o
+               Q.SPECL [`s`,`(\v. v = toy2set'' y s)`])
+  \\ FULL_SIMP_TAC bool_ss [SPLIT_toy2set_EXISTS]
+  \\ IMP_RES_TAC toy2set''_11 \\ Q.EXISTS_TAC `i` \\ METIS_TAC []);
+
+
+(* ----------------------------------------------------------------------------- *)
+(* Theorems for construction of |- SPEC TOY_MODEL ...                            *)
+(* ----------------------------------------------------------------------------- *)
+
+val STAR_toy2set = store_thm("STAR_toy2set",
+  ``((tRunstate y * p) (toy2set' (rs,pc,is,rg,fl,cc) s) <=>
+      y = s.runstate /\ rs /\ p (toy2set' (F,pc,is,rg,fl,cc) s)) /\
+    ((tPC v * p) (toy2set' (rs,pc,is,rg,fl,cc) s) <=>
+      v = s.pc /\ pc /\ p (toy2set' (rs,F,is,rg,fl,cc) s)) /\
+    ((tContext x1 x2 x3 * p) (toy2set' (rs,pc,is,rg,fl,cc) s) <=>
+      x1 = s.mload /\ x2 = s.mstore /\ x3 = s.context /\ cc /\
+      p (toy2set' (rs,pc,is,rg,fl,F) s)) /\
+    ((tFlag f x * p) (toy2set' (rs,pc,is,rg,fl,cc) s) <=>
+      (x = toy_read_flag f s) /\ f IN fl /\
+      p (toy2set' (rs,pc,is,rg,fl DELETE f,cc) s)) /\
+    ((tReg r w * p) (toy2set' (rs,pc,is,rg,fl,cc) s) <=>
+      (w = toy_read_reg r s) /\ r IN rg /\
+      p (toy2set' (rs,pc,is,rg DELETE r,fl,cc) s)) /\
+    ((tInst n i * p) (toy2set' (rs,pc,is,rg,fl,cc) s) <=>
+      (i = toy_read_inst n s) /\ n IN is /\
+      p (toy2set' (rs,pc,is DELETE n,rg,fl,cc) s))``,
+  SIMP_TAC std_ss [tRunstate_def, tPC_def, tInst_def, tReg_def,
+    tFlag_def, tContext_def, EQ_STAR, INSERT_SUBSET, cond_STAR,
+    EMPTY_SUBSET, IN_toy2set, GSYM DELETE_DEF]
+  \\ rpt strip_tac \\ eq_tac \\ rw [] \\ fs []);
+
+val tFlags_HIDE = store_thm("tFlags_HIDE",
+  ``~tFlags = ~tFlag ZF * ~tFlag SF``,
+  SIMP_TAC std_ss [SEP_HIDE_def,tFlag_def,SEP_CLAUSES,FUN_EQ_THM]
+  \\ SIMP_TAC std_ss [SEP_EXISTS,tFlag_def,EXISTS_PROD,Flags_def]);
+
+val TOY_SPEC_CODE =
+  SPEC_CODE |> ISPEC ``TOY_MODEL``
+  |> SIMP_RULE std_ss [TOY_MODEL_def]
+  |> RW [GSYM TOY_MODEL_def]
+  |> Q.SPECL [`p`,`{(a,x)}`,`q`] |> GSYM
+  |> SIMP_RULE std_ss [CODE_POOL_def,IMAGE_INSERT,IMAGE_EMPTY,BIGUNION_SING,
+        TOY_INSTR_def,GSYM (RW [SEP_EQ_def] tInst_def),TOY_SPEC_SEMANTICS]
+
+val IMP_TOY_SPEC_LEMMA = prove(
+  ``!a x p q.
+      (!rs pc is rg fl cc s.
+        (tInst a (SOME x) * p * emp) (toy2set' (rs,pc,is,rg,fl,cc) s) ==>
+        (tInst a (SOME x) * q * emp) (toy2set' (rs,pc,is,rg,fl,cc) (step s)) /\
+        (toy2set'' (rs,pc,is,rg,fl,cc) s =
+         toy2set'' (rs,pc,is,rg,fl,cc) (step s))) ==>
+      SPEC TOY_MODEL p {(a,x)} q``,
+  fs [TOY_SPEC_CODE,SEP_CLAUSES]
+  \\ SIMP_TAC std_ss [RIGHT_EXISTS_IMP_THM] \\ REWRITE_TAC [TOY_SPEC_SEMANTICS]
+  \\ rpt strip_tac
+  \\ PairCases_on `y` \\ RES_TAC
+  \\ FULL_SIMP_TAC bool_ss [rel_sequence_def,TOY_NEXT_REL_def]
+  \\ Q.EXISTS_TAC `SUC 0` \\ METIS_TAC [PAIR,optionTheory.SOME_11]);
+
+val PC_def = Define `TOY_PC p = tPC p * tRunstate RUNNING`;
+val _ = overload_on("PC",``TOY_PC``)
+
+val SOME_EQ_toy_read_inst_IFF = prove(
+  ``SOME x = toy_read_inst s.pc s <=>
+    s.pc < LENGTH s.instructions /\ EL s.pc s.instructions = x``,
+  fs [toy_read_inst_def]);
+
+val IS_SOME_EQ = prove(
+  ``IS_SOME x <=> ?b. x = SOME b``,
+  Cases_on `x` \\ fs []);
+
+(* MOV *)
+
+val MOV_CNST = store_thm("MOV_CNST",
+  ``SPEC TOY_MODEL
+      (PC p * tReg r w * tFlag ZF zf * tFlag SF n)
+      {(p,MOV r (CNST v))}
+      (PC (p+1) * tReg r v * tFlag ZF (v = 0w) * tFlag SF (word_msb v))``,
+  match_mp_tac IMP_TOY_SPEC_LEMMA
+  \\ fs [GSYM STAR_ASSOC,STAR_toy2set,PC_def]
+  \\ fs [emp_def] \\ rw []
+  \\ fs [step_def,SOME_EQ_toy_read_inst_IFF]
+  \\ fs [toy_read_inst_def,toy_read_reg_def,toy_read_flag_def,
+         flag_update_def,eval_regc_def,APPLY_UPDATE_THM]
+  THEN1 (Cases_on `r` \\ fs [fcpTheory.FCP_BETA,fcpTheory.FCP_UPDATE_def] \\ EVAL_TAC)
+  \\ simp [EXTENSION]
+  \\ Cases
+  \\ fs [toy_read_inst_def,toy_read_reg_def,toy_read_flag_def,flag_update_def,
+         eval_regc_def]
+  THEN1 (Cases_on `c` \\ fs [fcpTheory.FCP_BETA,fcpTheory.FCP_UPDATE_def] \\ EVAL_TAC
+         \\ rw [] \\ fs [])
+  \\ Cases_on `f` \\ fs [APPLY_UPDATE_THM] \\ rw []);
+
+val MOV_REG = store_thm("MOV_REG",
+  ``SPEC TOY_MODEL
+      (PC p * tReg r w * tReg r1 v * tFlag ZF zf * tFlag SF n)
+      {(p,MOV r (REG r1))}
+      (PC (p+1) * tReg r v * tReg r1 v * tFlag ZF (v = 0w) * tFlag SF (word_msb v))``,
+  match_mp_tac IMP_TOY_SPEC_LEMMA
+  \\ fs [GSYM STAR_ASSOC,STAR_toy2set,PC_def]
+  \\ fs [emp_def] \\ rw []
+  \\ fs [step_def,SOME_EQ_toy_read_inst_IFF]
+  \\ fs [toy_read_inst_def,toy_read_reg_def,toy_read_flag_def,
+         flag_update_def,eval_regc_def,APPLY_UPDATE_THM]
+  THEN1 (Cases_on `r` \\ fs [fcpTheory.FCP_BETA,fcpTheory.FCP_UPDATE_def] \\ EVAL_TAC)
+  THEN1 (Cases_on `r1` \\ fs [fcpTheory.FCP_BETA,fcpTheory.FCP_UPDATE_def])
+  \\ simp [EXTENSION]
+  \\ Cases
+  \\ fs [toy_read_inst_def,toy_read_reg_def,toy_read_flag_def,flag_update_def,
+         eval_regc_def]
+  THEN1 (Cases_on `c` \\ fs [fcpTheory.FCP_BETA,fcpTheory.FCP_UPDATE_def] \\ EVAL_TAC
+         \\ rw [] \\ fs [])
+  \\ Cases_on `f` \\ fs [APPLY_UPDATE_THM] \\ rw []);
+
+(* ILOAD *)
+
+val ILOAD = store_thm("ILOAD",
+  ``SPEC TOY_MODEL
+      (PC p * tReg a0 r0 * tReg a1 r1 * tContext mload mstore ctxt *
+       cond (IS_SOME (mload r1 ctxt)))
+      {(p,ILOAD a0 a1)}
+      (PC (p+1) * tReg a0 (FST (THE (mload r1 ctxt))) * tReg a1 r1 *
+       tContext mload mstore (SND (THE (mload r1 ctxt))))``,
+  fs [SPEC_MOVE_COND] \\ strip_tac
+  \\ match_mp_tac IMP_TOY_SPEC_LEMMA
+  \\ fs [GSYM STAR_ASSOC,STAR_toy2set,PC_def]
+  \\ fs [emp_def] \\ rw []
+  \\ fs [step_def,SOME_EQ_toy_read_inst_IFF]
+  \\ fs [toy_read_inst_def,toy_read_reg_def,toy_read_flag_def,
+         flag_update_def,eval_regc_def,APPLY_UPDATE_THM,IS_SOME_EQ]
+  \\ TRY (PairCases_on `b` \\ fs [])
+  THEN1 (Cases_on `a0`
+     \\ fs [fcpTheory.FCP_BETA,fcpTheory.FCP_UPDATE_def] \\ EVAL_TAC)
+  THEN1 (Cases_on `a1` \\ Cases_on `a0`
+     \\ fs [fcpTheory.FCP_BETA,fcpTheory.FCP_UPDATE_def] \\ EVAL_TAC)
+  \\ simp [EXTENSION]
+  \\ Cases
+  \\ fs [toy_read_inst_def,toy_read_reg_def,toy_read_flag_def,flag_update_def,
+         eval_regc_def]
+  \\ Cases_on `c` \\ Cases_on `a0`
+  \\ fs [fcpTheory.FCP_BETA,fcpTheory.FCP_UPDATE_def] \\ EVAL_TAC
+  \\ rw [] \\ fs [])
+
+val ILOAD' = store_thm("ILOAD'",
+  ``SPEC TOY_MODEL
+      (PC p * tReg a0 r0 * tContext mload mstore ctxt *
+       cond (IS_SOME (mload r0 ctxt)))
+      {(p,ILOAD a0 a0)}
+      (PC (p+1) * tReg a0 (FST (THE (mload r0 ctxt))) *
+       tContext mload mstore (SND (THE (mload r0 ctxt))))``,
+  fs [SPEC_MOVE_COND] \\ strip_tac
+  \\ match_mp_tac IMP_TOY_SPEC_LEMMA
+  \\ fs [GSYM STAR_ASSOC,STAR_toy2set,PC_def]
+  \\ fs [emp_def] \\ rw []
+  \\ fs [step_def,SOME_EQ_toy_read_inst_IFF]
+  \\ fs [toy_read_inst_def,toy_read_reg_def,toy_read_flag_def,
+         flag_update_def,eval_regc_def,APPLY_UPDATE_THM,IS_SOME_EQ]
+  \\ TRY (PairCases_on `b` \\ fs [])
+  THEN1 (Cases_on `a0`
+     \\ fs [fcpTheory.FCP_BETA,fcpTheory.FCP_UPDATE_def] \\ EVAL_TAC)
+  \\ simp [EXTENSION]
+  \\ Cases
+  \\ fs [toy_read_inst_def,toy_read_reg_def,toy_read_flag_def,flag_update_def,
+         eval_regc_def]
+  \\ Cases_on `c` \\ Cases_on `a0`
+  \\ fs [fcpTheory.FCP_BETA,fcpTheory.FCP_UPDATE_def] \\ EVAL_TAC
+  \\ rw [] \\ fs []);
+
+(* ISTORE *)
+
+val ISTORE = store_thm("ISTORE",
+  ``SPEC TOY_MODEL
+      (PC p * tReg a0 r0 * tReg a1 r1 * tContext mload mstore ctxt *
+       cond (IS_SOME (mstore r0 r1 ctxt)))
+      {(p,ISTORE a1 a0)}
+      (PC (p+1) * tReg a0 r0 * tReg a1 r1 *
+       tContext mload mstore (THE (mstore r0 r1 ctxt)))``,
+  fs [SPEC_MOVE_COND] \\ strip_tac
+  \\ match_mp_tac IMP_TOY_SPEC_LEMMA
+  \\ fs [GSYM STAR_ASSOC,STAR_toy2set,PC_def]
+  \\ fs [emp_def] \\ rw []
+  \\ fs [step_def,SOME_EQ_toy_read_inst_IFF]
+  \\ fs [toy_read_inst_def,toy_read_reg_def,toy_read_flag_def,
+         flag_update_def,eval_regc_def,APPLY_UPDATE_THM,IS_SOME_EQ]
+  \\ simp [EXTENSION] \\ Cases
+  \\ fs [toy_read_inst_def,toy_read_reg_def,toy_read_flag_def,flag_update_def,
+         eval_regc_def]);
+
+val ISTORE' = store_thm("ISTORE'",
+  ``SPEC TOY_MODEL
+      (PC p * tReg a0 r0 * tContext mload mstore ctxt *
+       cond (IS_SOME (mstore r0 r0 ctxt)))
+      {(p,ISTORE a0 a0)}
+      (PC (p+1) * tReg a0 r0 *
+       tContext mload mstore (THE (mstore r0 r0 ctxt)))``,
+  fs [SPEC_MOVE_COND] \\ strip_tac
+  \\ match_mp_tac IMP_TOY_SPEC_LEMMA
+  \\ fs [GSYM STAR_ASSOC,STAR_toy2set,PC_def]
+  \\ fs [emp_def] \\ rw []
+  \\ fs [step_def,SOME_EQ_toy_read_inst_IFF]
+  \\ fs [toy_read_inst_def,toy_read_reg_def,toy_read_flag_def,
+         flag_update_def,eval_regc_def,APPLY_UPDATE_THM,IS_SOME_EQ]
+  \\ simp [EXTENSION] \\ Cases
+  \\ fs [toy_read_inst_def,toy_read_reg_def,toy_read_flag_def,flag_update_def,
+         eval_regc_def]);
+
+val _ = export_theory();
